Add addr_domain's missing SilcLabel case; WIP on TA subset inv forms
Signed-off-by: Robert Sison <robert.sison@unimelb.edu.au>

proof/infoflow/timeprotection/TimeProtectionIntegration.thy
@@ -19,11 +19,16 @@ type_synonym if_other_state    = "context_and_state \<times> sys_mode"
 (* note the 64 word it takes is a *physical address*. *)
 definition addr_domain where
   "addr_domain initial_aag pa \<equiv> case pasObjectAbs initial_aag ((inv RISCV64.addrFromKPPtr) pa) of
-     OrdinaryLabel l \<Rightarrow> Partition l"
+     OrdinaryLabel l \<Rightarrow> Partition l | SilcLabel \<Rightarrow> PSched"
 
+(* FIXME: addr_colour shouldn't even actually be consulting the policy.
+   Instead we should specify an address-to-colour assignment and prove that it lines up with
+   the policy. Case in point: We'll never know what the colour will be simply from knowing
+   we're talking about a SilcLabel! We can only know it from the addr-to-colour assignment,
+   which is what this parameter is supposed to be! -robs *)
 definition addr_colour where
   "addr_colour initial_aag pa \<equiv> case pasObjectAbs initial_aag ((inv RISCV64.addrFromKPPtr) pa) of
-     OrdinaryLabel l \<Rightarrow> l"
+     OrdinaryLabel l \<Rightarrow> l | SilcLabel \<Rightarrow> undefined"
 
 definition colour_userdomain where
   "colour_userdomain \<equiv> Partition"
@@ -940,20 +945,62 @@ interpretation l2p?: ArchL2Partitioned "TYPE('l subject_label \<times> 'l)"
   "\<lambda>sl. case sl of OrdinaryLabel l \<Rightarrow> l"
   done
 
-(* FIXME: Type errors between `'l subject_label` and `'l` are fixed, but we still need to
-   reconcile the following two forms of touched_addrs_inv. Form 1: *)
+lemma ta_vaddr_to_paddr:
+  "snd ` ii.touched_addresses s =
+   addrFromKPPtr ` machine_state.touched_addresses (machine_state (snd $ fst s))"
+  unfolding touched_addresses_def touched_vaddrs_def image_def
+  apply(clarsimp split:vaddr.splits)
+  apply(rule set_eqI)
+  apply clarsimp
+  by (metis vaddr.exhaust vaddr.inject)
+
+(* FIXME: Finish proving correspondence between "invariant lemmas" and "locale" form
+   of the ta subset invariant. *)
+lemma accessible_vaddr_to_paddr:
+  "all_paddrs_of (userPart s) \<union> kernel_shared_precise =
+   addrFromKPPtr ` pas_addrs_accessible_to initial_aag (cur_label initial_aag (snd $ fst s))"
+  unfolding all_paddrs_of_def kernel_shared_precise_def
+  unfolding addr_domain_def
+  apply(clarsimp simp:userPart_def)
+  apply(clarsimp split:subject_label.splits)
+  apply(rule set_eqI)
+  apply clarsimp
+  apply(clarsimp simp:image_def)
+  unfolding pas_addrs_accessible_to_def pas_labels_accessible_to_def
+  apply clarsimp
+  apply(rule iffI)
+   (* Case: vaddr version of accessibility implies paddr one *)
+   apply(erule disjE)
+    apply clarsimp
+    defer
+   defer
+  (* Case: paddr version of accessibility implies vaddr one *)
+  apply clarsimp
+  sorry
+
+thm ta_subset_inv_def touched_addrs_inv_def
+lemma ta_subset_inv_to_locale_form:
+  "l2p.ta_subset_inv initial_aag (snd $ fst s) \<Longrightarrow>
+  touched_addrs_inv s"
+  unfolding touched_addrs_inv_def
+  unfolding ta_subset_inv_def
+  apply(clarsimp simp: ta_vaddr_to_paddr accessible_vaddr_to_paddr)
+  apply(clarsimp simp:image_def)
+  by blast
+
 thm ta_subset_inv_def
-lemma l2p_subset_inv_form:
+lemma ta_subset_inv_reachable:
+  (* According to Scott, initial_aag should be fine here rather than `current_aag (snd $ fst s0)` *)
   "reachable s \<Longrightarrow>
-  l2p.ta_subset_inv (current_aag (snd $ fst so)) (snd $ fst s)"
+  l2p.ta_subset_inv initial_aag (snd $ fst s)"
   subgoal sorry
   done
 
-(* FIXME: Form 2: *)
 lemma subset_inv_proof:
   "reachable s \<Longrightarrow>
   touched_addrs_inv s"
-  sorry (* FIXME: needs to be somehow derived from l2-_subset_inv or something *)
+  using ta_subset_inv_reachable ta_subset_inv_to_locale_form
+  by blast
 
 (* I don't think this should be too bad. Can do this with hoare logic stuff I think. *)
 lemma domainswitch_follows_get_next_domain:
